remove ateq and iateq

yalla/isubs.v
@@ -10,23 +10,17 @@ Section Atoms.
 
 Context {preiatom : InfDecType}.
 Notation atN := (@atN preiatom).
-Definition iateq := @eqb (option_dectype preiatom).
-Definition iateq_eq := @eqb_eq (option_dectype preiatom).
 
 (** ** Substitutions *)
 
 (** basic operation for substitution of atoms *)
-Definition repl_iat x y A := if iateq x y then A else ivar x.
+Definition repl_iat x y A := if (@eq_dt_dec (option_dectype preiatom) x y) then A else ivar x.
 
-Lemma repl_iat_eq x y A : x = y -> repl_iat x y A = A.
-Proof. intros ->. unfold repl_iat. rewrite (proj2 (iateq_eq _ _) (eq_refl _)). reflexivity. Qed.
+Lemma repl_iat_eq x A : repl_iat x x A = A.
+Proof. unfold repl_iat. rewrite if_eq_dt_dec_refl. reflexivity. Qed.
 
 Lemma repl_iat_neq x y A : x <> y -> repl_iat x y A = ivar x.
-Proof.
-intros Hneq. unfold repl_iat.
-destruct (iateq x y) eqn:Heqb; [ exfalso | reflexivity ].
-rewrite iateq_eq in Heqb. contradiction Heqb.
-Qed.
+Proof. intros Hneq. unfold repl_iat. rewrite (if_eq_dt_dec_neq _ Hneq). reflexivity. Qed.
 
 (** Substitution in [iformula]: substitutes [x] by [C] in [A] *)
 Fixpoint isubs C x A :=
@@ -35,25 +29,24 @@ match A with
 | ione      => ione
 | itens A B => itens (isubs C x A) (isubs C x B)
 | ilpam A B => ilpam (isubs C x A) (isubs C x B)
-| igen A => igen (isubs C x A)
+| igen A    => igen (isubs C x A)
 | ilmap A B => ilmap (isubs C x A) (isubs C x B)
-| ineg A => ineg (isubs C x A)
-| izero => izero
-| itop => itop
+| ineg A    => ineg (isubs C x A)
+| izero     => izero
+| itop      => itop
 | iplus A B => iplus (isubs C x A) (isubs C x B)
 | iwith A B => iwith (isubs C x A) (isubs C x B)
 | ioc A     => ioc (isubs C x A)
 end.
 
 (** Substitution in proofs *)
-Lemma subs_ill P A x l C (HN : x <> atN) (Hcut : forall D, Bool.le (ipcut P D) (ipcut P (isubs A x D))) :
+Lemma subs_ill P A x l C (HN : atN <> x) (Hcut : forall D, Bool.le (ipcut P D) (ipcut P (isubs A x D))) :
   ill P l C ->
   ill (axupd_ipfrag P (existT (fun x => x -> list iformula * iformula) _
                               (fun a => (map (isubs A x) (fst (projT2 (ipgax P) a)),
                                              isubs A x (snd (projT2 (ipgax P) a))))))
       (map (isubs A x) l) (isubs A x C).
 Proof.
-apply <- (@eqb_neq (option_dectype preiatom)) in HN. rewrite eqb_sym in HN. fold iateq in HN.
 intros pi.
 assert (forall l, map (isubs A x) (map ioc l) = map ioc (map (isubs A x) l)) as Hmapioc
   by (clear; induction l as [|a l IHl]; [ | cbn; rewrite IHl ]; reflexivity).
@@ -69,10 +62,10 @@ induction pi; cbn; rewrite ? map_app;
   eapply Permutation_Type_map in p.
   eapply ex_oc_ir; eassumption.
 - list_simpl. apply lpam_ilr; assumption.
-- unfold repl_iat in IHpi. rewrite HN in IHpi. apply gen_irr. assumption.
-- unfold repl_iat. rewrite HN. apply gen_ilr. assumption.
-- unfold repl_iat in IHpi. rewrite HN in IHpi. apply neg_irr. assumption.
-- unfold repl_iat. rewrite HN. apply neg_ilr. assumption.
+- unfold repl_iat in IHpi. rewrite if_eq_dt_dec_neq in IHpi by exact HN. apply gen_irr, IHpi.
+- unfold repl_iat. rewrite if_eq_dt_dec_neq by exact HN. apply gen_ilr, IHpi.
+- unfold repl_iat in IHpi. rewrite if_eq_dt_dec_neq in IHpi by exact HN. apply neg_irr, IHpi.
+- unfold repl_iat. rewrite if_eq_dt_dec_neq by exact HN. apply neg_ilr, IHpi.
 - specialize Hmapioc with l.
   rewrite Hmapioc. apply oc_irr. rewrite <- Hmapioc. assumption.
 - refine (cut_ir (isubs A x A0) _ IHpi1 IHpi2).
@@ -82,7 +75,7 @@ induction pi; cbn; rewrite ? map_app;
 Qed.
 
 Lemma subs_ill_axfree P (P_axfree : notT (projT1 (ipgax P))) A x
-  (Hcut : forall D, Bool.le (ipcut P D) (ipcut P (isubs A x D))) l C (HN : x <> atN) :
+  (Hcut : forall D, Bool.le (ipcut P D) (ipcut P (isubs A x D))) l C (HN : atN <> x) :
   ill P l C -> ill P (map (isubs A x) l) (isubs A x C).
 Proof.
 intros pi.
